TCB/BinaryDefs.v
@@ -1,0 +1,117 @@
+Require Import Lib.
+Open Scope positive_scope.
+Open Scope N_scope.
+
+
+(* Definition of a half byte *)
+
+Inductive half_byte :=
+| HB0
+| HB1
+| HB2
+| HB3
+| HB4
+| HB5
+| HB6
+| HB7
+| HB8
+| HB9
+| HBA
+| HBB
+| HBC
+| HBD
+| HBE
+| HBF.
+
+
+
+Definition half_byte_to_N hb : N:=
+  match hb with
+    | HB0 => 0
+    | HB1 => 1
+    | HB2 => 2
+    | HB3 => 3
+    | HB4 => 4
+    | HB5 => 5
+    | HB6 => 6
+    | HB7 => 7
+    | HB8 => 8
+    | HB9 => 9
+    | HBA => 10
+    | HBB => 11
+    | HBC => 12
+    | HBD => 13
+    | HBE => 14
+    | HBF => 15
+  end.
+
+(* add [trans] 0 bits *)
+
+Fixpoint translate_P_by trans (p: positive) :=
+  match trans with
+    | O => p
+    | S t' => translate_P_by t' (p~0)
+  end.
+
+Definition translate_N_by trans (n: N) :=
+  match n with
+    | N0 => N0
+    | Npos p => Npos (translate_P_by trans p)
+  end.
+
+(* specialisation for efficiency reasons *)
+Definition translate_N_by_four n :=
+  match n with
+    | N0 => N0
+    | Npos p => Npos (p~0~0~0~0)
+  end.
+
+Definition translate_N_by_eight n :=
+  match n with
+    | 0 => 0
+    | Npos p => Npos (p~0~0~0~0~0~0~0~0)
+  end.
+
+Lemma translate_N_by_four_correct: forall n, translate_N_by_four n = translate_N_by 4 n.
+Proof.
+  intros [|pos]; reflexivity.
+Qed.
+
+Lemma translate_N_by_eight_correct: forall n, translate_N_by_eight n = translate_N_by 8 n.
+Proof.
+  intros [|pos]; reflexivity.
+Qed.
+
+
+Definition concat_half_byte n hb := (translate_N_by_four n) + (half_byte_to_N hb).
+
+
+
+
+
+(* Bytes *)
+
+Definition byte := (half_byte * half_byte)%type.
+
+Definition byte_to_N (b: byte) : N:=
+  concat_half_byte (half_byte_to_N (fst b)) (snd b).
+
+Definition byte0 : byte := (HB0, HB0).
+
+
+Definition concat_byte n (b: byte) :=
+  translate_N_by_eight n + byte_to_N b.
+
+
+(* a word is four byte, little endian *)
+Inductive word := W : byte -> byte -> byte -> byte -> word.
+
+Definition word_to_N w :=
+  match w with
+    | W b1 b2 b3 b4 =>
+      let n4 := byte_to_N b4 in
+      let n3 := concat_byte n4 b3 in
+      let n2 := concat_byte n3 b2 in
+      concat_byte n2 b1
+  end.
+
