TCB/BinaryProps.v
@@ -1,0 +1,33 @@
+Require Import Lib.
+Require Import BinaryDefs.
+Require Import BinaryAux.
+Open Scope positive_scope.
+Open Scope N_scope.
+
+
+Lemma byte_to_N0: byte_to_N byte0 = 0.
+Proof.
+  reflexivity.
+Qed.
+
+Lemma fst_byte_of_byte: forall b n,
+  fst_byte (concat_byte n b) = (b, n).
+Proof.
+  intros.
+  rewrite concat_byte_aux_correct.
+  destruct b as (hb2, hb1).
+  unfold fst_byte.
+  simpl.
+  repeat rewrite fst_four_bits_of_half_byte. reflexivity.
+Qed.
+
+Lemma fst_word_of_word: forall w,
+  to_word (word_to_N w) = w.
+Proof.
+  destruct w as [b1 b2 b3 b4].
+  unfold to_word.
+  simpl. repeat rewrite fst_byte_of_byte.
+  unfold fst_byte, byte_to_N.
+  rewrite fst_four_bits_of_half_byte.
+  destruct b4. simpl. destruct h; reflexivity.
+Qed.
